Revert "Merge branch 'swasey/progress' into 'master'"
This reverts commit 849abb8da669d524294a912fc20cf7e450e38fb3, reversing changes
made to 8de0b89477d103cda42f16dade7f5a8e103522bd.  The merge was done
accidentally, before review happened.

theories/program_logic/language.v
@@ -43,20 +43,6 @@ Class LanguageCtx (Λ : language) (K : expr Λ → expr Λ) := {
 Instance language_ctx_id Λ : LanguageCtx Λ id.
 Proof. constructor; naive_solver. Qed.
 
-Variant stuckness := not_stuck | maybe_stuck.
-Definition stuckness_le (s1 s2 : stuckness) : bool :=
-  match s1, s2 with
-  | maybe_stuck, not_stuck => false
-  | _, _ => true
-  end.
-Instance: @PreOrder stuckness stuckness_le.
-Proof.
-  split; first by case. move=>s1 s2 s3. by case: s1; case: s2; case: s3.
-Qed.
-Bind Scope stuckness_scope with stuckness.
-Delimit Scope stuckness_scope with stuckness.
-Infix "≤" := stuckness_le : stuckness_scope.
-
 Section language.
   Context {Λ : language}.
   Implicit Types v : val Λ.
@@ -65,24 +51,22 @@ Section language.
     ∃ e' σ' efs, prim_step e σ e' σ' efs.
   Definition irreducible (e : expr Λ) (σ : state Λ) :=
     ∀ e' σ' efs, ¬prim_step e σ e' σ' efs.
-  Definition progressive (e : expr Λ) (σ : state Λ) :=
-    is_Some (to_val e) ∨ reducible e σ.
 
-  (* [Atomic not_stuck]: This (weak) form of atomicity is enough to open invariants when WP ensures
+  (* This (weak) form of atomicity is enough to open invariants when WP ensures
      safety, i.e., programs never can get stuck.  We have an example in
      lambdaRust of an expression that is atomic in this sense, but not in the
      stronger sense defined below, and we have to be able to open invariants
      around that expression.  See `CasStuckS` in
-     [lambdaRust](https://gitlab.mpi-sws.org/FP/LambdaRust-coq/blob/master/theories/lang/lang.v).
+     [lambdaRust](https://gitlab.mpi-sws.org/FP/LambdaRust-coq/blob/master/theories/lang/lang.v). *)
+  Class Atomic (e : expr Λ) : Prop :=
+    atomic σ e' σ' efs : prim_step e σ e' σ' efs → irreducible e' σ'.
 
-     [Atomic maybe_stuck]: To open invariants with a WP that does not ensure safety, we need a
+  (* To open invariants with a WP that does not ensure safety, we need a
      stronger form of atomicity.  With the above definition, in case `e` reduces
      to a stuck non-value, there is no proof that the invariants have been
      established again. *)
-  Class Atomic (s : stuckness) (e : expr Λ) : Prop :=
-    atomic σ e' σ' efs :
-      prim_step e σ e' σ' efs →
-      if s is not_stuck then irreducible e' σ' else is_Some (to_val e').
+  Class StronglyAtomic (e : expr Λ) : Prop :=
+    strongly_atomic σ e' σ' efs : prim_step e σ e' σ' efs → is_Some (to_val e').
 
   Inductive step (ρ1 ρ2 : cfg Λ) : Prop :=
     | step_atomic e1 σ1 e2 σ2 efs t1 t2 :
@@ -103,8 +87,8 @@ Section language.
   Global Instance of_val_inj : Inj (=) (=) (@of_val Λ).
   Proof. by intros v v' Hv; apply (inj Some); rewrite -!to_of_val Hv. Qed.
 
-  Lemma strongly_atomic_atomic e : Atomic maybe_stuck e → Atomic not_stuck e.
-  Proof. unfold Atomic. eauto using val_irreducible. Qed.
+  Lemma strongly_atomic_atomic e : StronglyAtomic e → Atomic e.
+  Proof. unfold StronglyAtomic, Atomic. eauto using val_irreducible. Qed.
 
   Lemma reducible_fill `{LanguageCtx Λ K} e σ :
     to_val e = None → reducible (K e) σ → reducible e σ.
