theories/program_logic/ectx_lifting.v
@@ -6,94 +6,67 @@ Set Default Proof Using "Type".
 Section wp.
 Context {expr val ectx state} {Λ : EctxLanguage expr val ectx state}.
 Context `{irisG (ectx_lang expr) Σ} {Hinh : Inhabited state}.
-Implicit Types s : stuckness.
 Implicit Types P : iProp Σ.
 Implicit Types Φ : val → iProp Σ.
 Implicit Types v : val.
 Implicit Types e : expr.
 Hint Resolve head_prim_reducible head_reducible_prim_step.
-Hint Resolve (reducible_not_val _ inhabitant).
-Hint Resolve progressive_head_progressive.
 
-Lemma wp_ectx_bind {s E e} K Φ :
-  WP e @ s; E {{ v, WP fill K (of_val v) @ s; E {{ Φ }} }}
-  ⊢ WP fill K e @ s; E {{ Φ }}.
+Lemma wp_ectx_bind {E Φ} K e :
+  WP e @ E {{ v, WP fill K (of_val v) @ E {{ Φ }} }} ⊢ WP fill K e @ E {{ Φ }}.
 Proof. apply: weakestpre.wp_bind. Qed.
 
-Lemma wp_ectx_bind_inv {s E Φ} K e :
-  WP fill K e @ s; E {{ Φ }}
-  ⊢ WP e @ s; E {{ v, WP fill K (of_val v) @ s; E {{ Φ }} }}.
+Lemma wp_ectx_bind_inv {E Φ} K e :
+  WP fill K e @ E {{ Φ }} ⊢ WP e @ E {{ v, WP fill K (of_val v) @ E {{ Φ }} }}.
 Proof. apply: weakestpre.wp_bind_inv. Qed.
 
-Lemma wp_lift_head_step {s E Φ} e1 :
+Lemma wp_lift_head_step {E Φ} e1 :
   to_val e1 = None →
   (∀ σ1, state_interp σ1 ={E,∅}=∗
     ⌜head_reducible e1 σ1⌝ ∗
     ▷ ∀ e2 σ2 efs, ⌜head_step e1 σ1 e2 σ2 efs⌝ ={∅,E}=∗
-      state_interp σ2 ∗ WP e2 @ s; E {{ Φ }} ∗ [∗ list] ef ∈ efs, WP ef @ s; ⊤ {{ _, True }})
-  ⊢ WP e1 @ s; E {{ Φ }}.
+      state_interp σ2 ∗ WP e2 @ E {{ Φ }} ∗ [∗ list] ef ∈ efs, WP ef {{ _, True }})
+  ⊢ WP e1 @ E {{ Φ }}.
 Proof.
-  iIntros (?) "H". iApply wp_lift_step=>//. iIntros (σ1) "Hσ".
-  iMod ("H" with "Hσ") as "[% H]"; iModIntro.
-  iSplit; first by destruct s; eauto. iNext. iIntros (e2 σ2 efs) "%".
-  iApply "H"; eauto.
+  iIntros (?) "H". iApply (wp_lift_step E)=>//. iIntros (σ1) "Hσ".
+  iMod ("H" $! σ1 with "Hσ") as "[% H]"; iModIntro.
+  iSplit; first by eauto. iNext. iIntros (e2 σ2 efs) "%".
+  iApply "H". by eauto.
 Qed.
 
-Lemma wp_lift_head_stuck E Φ e :
-  to_val e = None →
-  (∀ σ, state_interp σ ={E,∅}=∗ ⌜¬ head_progressive e σ⌝)
-  ⊢ WP e @ E ?{{ Φ }}.
-Proof.
-  iIntros (?) "H". iApply wp_lift_stuck; first done.
-  iIntros (σ) "Hσ". iMod ("H" with "Hσ") as "%". by auto. 
-Qed.
-
-Lemma wp_lift_pure_head_step {s E E' Φ} e1 :
+Lemma wp_lift_pure_head_step {E E' Φ} e1 :
   (∀ σ1, head_reducible e1 σ1) →
   (∀ σ1 e2 σ2 efs, head_step e1 σ1 e2 σ2 efs → σ1 = σ2) →
   (|={E,E'}▷=> ∀ e2 efs σ, ⌜head_step e1 σ e2 σ efs⌝ →
-    WP e2 @ s; E {{ Φ }} ∗ [∗ list] ef ∈ efs, WP ef @ s; ⊤ {{ _, True }})
-  ⊢ WP e1 @ s; E {{ Φ }}.
+    WP e2 @ E {{ Φ }} ∗ [∗ list] ef ∈ efs, WP ef {{ _, True }})
+  ⊢ WP e1 @ E {{ Φ }}.
 Proof using Hinh.
   iIntros (??) "H". iApply wp_lift_pure_step; eauto.
-  { by destruct s; auto. }
   iApply (step_fupd_wand with "H"); iIntros "H".
   iIntros (????). iApply "H"; eauto.
 Qed.
 
-Lemma wp_lift_pure_head_stuck E Φ e :
-  to_val e = None →
-  (∀ K e1 σ1 e2 σ2 efs, e = fill K e1 → ¬ head_step e1 σ1 e2 σ2 efs) →
-  WP e @ E ?{{ Φ }}%I.
-Proof using Hinh.
-  iIntros (Hnv Hnstep). iApply wp_lift_head_stuck; first done.
-  iIntros (σ) "_". iMod (fupd_intro_mask' E ∅) as "_"; first set_solver.
-  iModIntro. iPureIntro. case; first by rewrite Hnv; case.
-  move=>[] K [] e1 [] Hfill [] e2 [] σ2 [] efs /= Hstep. exact: Hnstep.
-Qed.
-
-Lemma wp_lift_atomic_head_step {s E Φ} e1 :
+Lemma wp_lift_atomic_head_step {E Φ} e1 :
   to_val e1 = None →
   (∀ σ1, state_interp σ1 ={E}=∗
     ⌜head_reducible e1 σ1⌝ ∗
     ▷ ∀ e2 σ2 efs, ⌜head_step e1 σ1 e2 σ2 efs⌝ ={E}=∗
       state_interp σ2 ∗
-      default False (to_val e2) Φ ∗ [∗ list] ef ∈ efs, WP ef @ s; ⊤ {{ _, True }})
-  ⊢ WP e1 @ s; E {{ Φ }}.
+      default False (to_val e2) Φ ∗ [∗ list] ef ∈ efs, WP ef {{ _, True }})
+  ⊢ WP e1 @ E {{ Φ }}.
 Proof.
   iIntros (?) "H". iApply wp_lift_atomic_step; eauto.
-  iIntros (σ1) "Hσ1". iMod ("H" with "Hσ1") as "[% H]"; iModIntro.
-  iSplit; first by destruct s; auto. iNext. iIntros (e2 σ2 efs) "%".
-  iApply "H"; auto.
+  iIntros (σ1) "Hσ1". iMod ("H" $! σ1 with "Hσ1") as "[% H]"; iModIntro.
+  iSplit; first by eauto. iNext. iIntros (e2 σ2 efs) "%". iApply "H"; auto.
 Qed.
 
-Lemma wp_lift_atomic_head_step_no_fork {s E Φ} e1 :
+Lemma wp_lift_atomic_head_step_no_fork {E Φ} e1 :
   to_val e1 = None →
   (∀ σ1, state_interp σ1 ={E}=∗
     ⌜head_reducible e1 σ1⌝ ∗
     ▷ ∀ e2 σ2 efs, ⌜head_step e1 σ1 e2 σ2 efs⌝ ={E}=∗
       ⌜efs = []⌝ ∗ state_interp σ2 ∗ default False (to_val e2) Φ)
-  ⊢ WP e1 @ s; E {{ Φ }}.
+  ⊢ WP e1 @ E {{ Φ }}.
 Proof.
   iIntros (?) "H". iApply wp_lift_atomic_head_step; eauto.
   iIntros (σ1) "Hσ1". iMod ("H" $! σ1 with "Hσ1") as "[$ H]"; iModIntro.
@@ -101,29 +74,25 @@ Proof.
   iMod ("H" $! v2 σ2 efs with "[# //]") as "(% & $ & $)"; subst; auto.
 Qed.
 
-Lemma wp_lift_pure_det_head_step {s E E' Φ} e1 e2 efs :
+Lemma wp_lift_pure_det_head_step {E E' Φ} e1 e2 efs :
   (∀ σ1, head_reducible e1 σ1) →
   (∀ σ1 e2' σ2 efs',
     head_step e1 σ1 e2' σ2 efs' → σ1 = σ2 ∧ e2 = e2' ∧ efs = efs') →
-  (|={E,E'}▷=> WP e2 @ s; E {{ Φ }} ∗ [∗ list] ef ∈ efs, WP ef @ s; ⊤ {{ _, True }})
-  ⊢ WP e1 @ s; E {{ Φ }}.
-Proof using Hinh.
-  intros. rewrite -(wp_lift_pure_det_step e1 e2 efs); eauto.
-  destruct s; by auto.
-Qed.
+  (|={E,E'}▷=> WP e2 @ E {{ Φ }} ∗ [∗ list] ef ∈ efs, WP ef {{ _, True }})
+  ⊢ WP e1 @ E {{ Φ }}.
+Proof using Hinh. eauto using wp_lift_pure_det_step. Qed.
 
-Lemma wp_lift_pure_det_head_step_no_fork {s E E' Φ} e1 e2 :
+Lemma wp_lift_pure_det_head_step_no_fork {E E' Φ} e1 e2 :
   to_val e1 = None →
   (∀ σ1, head_reducible e1 σ1) →
   (∀ σ1 e2' σ2 efs',
     head_step e1 σ1 e2' σ2 efs' → σ1 = σ2 ∧ e2 = e2' ∧ [] = efs') →
-  (|={E,E'}▷=> WP e2 @ s; E {{ Φ }}) ⊢ WP e1 @ s; E {{ Φ }}.
+  (|={E,E'}▷=> WP e2 @ E {{ Φ }}) ⊢ WP e1 @ E {{ Φ }}.
 Proof using Hinh.
   intros. rewrite -(wp_lift_pure_det_step e1 e2 []) /= ?right_id; eauto.
-  destruct s; by auto.
 Qed.
 
-Lemma wp_lift_pure_det_head_step_no_fork' {s E Φ} e1 e2 :
+Lemma wp_lift_pure_det_head_step_no_fork' {E Φ} e1 e2 :
   to_val e1 = None →
   (∀ σ1, head_reducible e1 σ1) →
   (∀ σ1 e2' σ2 efs',
