theories/program_logic/lifting.v
@@ -5,76 +5,50 @@ Set Default Proof Using "Type".
 
 Section lifting.
 Context `{irisG Λ Σ}.
-Implicit Types s : stuckness.
 Implicit Types v : val Λ.
 Implicit Types e : expr Λ.
 Implicit Types σ : state Λ.
 Implicit Types P Q : iProp Σ.
 Implicit Types Φ : val Λ → iProp Σ.
 
-Lemma wp_lift_step s E Φ e1 :
+Lemma wp_lift_step E Φ e1 :
   to_val e1 = None →
   (∀ σ1, state_interp σ1 ={E,∅}=∗
-    ⌜if s is not_stuck then reducible e1 σ1 else True⌝ ∗
+    ⌜reducible e1 σ1⌝ ∗
     ▷ ∀ e2 σ2 efs, ⌜prim_step e1 σ1 e2 σ2 efs⌝ ={∅,E}=∗
-      state_interp σ2 ∗ WP e2 @ s; E {{ Φ }} ∗ [∗ list] ef ∈ efs, WP ef @ s; ⊤ {{ _, True }})
-  ⊢ WP e1 @ s; E {{ Φ }}.
-Proof.
-  rewrite wp_unfold /wp_pre=>->. iIntros "H" (σ1) "Hσ".
-  iMod ("H" with "Hσ") as "(%&?)". iModIntro. iSplit. by destruct s. done.
-Qed.
-
-Lemma wp_lift_stuck E Φ e :
-  to_val e = None →
-  (∀ σ, state_interp σ ={E,∅}=∗ ⌜¬ progressive e σ⌝)
-  ⊢ WP e @ E ?{{ Φ }}.
-Proof.
-  rewrite wp_unfold /wp_pre=>->. iIntros "H" (σ1) "Hσ".
-  iMod ("H" with "Hσ") as "Hstuck". iDestruct "Hstuck" as %Hstuck.
-  iModIntro. iSplit; first done. iIntros "!>" (e2 σ2 efs) "%". exfalso.
-  apply Hstuck. right. by exists e2, σ2, efs.
-Qed.
+      state_interp σ2 ∗ WP e2 @ E {{ Φ }} ∗ [∗ list] ef ∈ efs, WP ef {{ _, True }})
+  ⊢ WP e1 @ E {{ Φ }}.
+Proof. by rewrite wp_unfold /wp_pre=> ->. Qed.
 
 (** Derived lifting lemmas. *)
-Lemma wp_lift_pure_step `{Inhabited (state Λ)} s E E' Φ e1 :
-  to_val e1 = None →
-  (∀ σ1, if s is not_stuck then reducible e1 σ1 else True) →
+Lemma wp_lift_pure_step `{Inhabited (state Λ)} E E' Φ e1 :
+  (∀ σ1, reducible e1 σ1) →
   (∀ σ1 e2 σ2 efs, prim_step e1 σ1 e2 σ2 efs → σ1 = σ2) →
   (|={E,E'}▷=> ∀ e2 efs σ, ⌜prim_step e1 σ e2 σ efs⌝ →
-    WP e2 @ s; E {{ Φ }} ∗ [∗ list] ef ∈ efs, WP ef @ s; ⊤ {{ _, True }})
-  ⊢ WP e1 @ s; E {{ Φ }}.
+    WP e2 @ E {{ Φ }} ∗ [∗ list] ef ∈ efs, WP ef {{ _, True }})
+  ⊢ WP e1 @ E {{ Φ }}.
 Proof.
-  iIntros (? Hsafe Hstep) "H". iApply wp_lift_step; first done.
+  iIntros (Hsafe Hstep) "H". iApply wp_lift_step.
+  { eapply reducible_not_val, (Hsafe inhabitant). }
   iIntros (σ1) "Hσ". iMod "H".
-  iMod fupd_intro_mask' as "Hclose"; last iModIntro; first by set_solver.
-  iSplit; first by iPureIntro; apply Hsafe. iNext. iIntros (e2 σ2 efs ?).
+  iMod fupd_intro_mask' as "Hclose"; last iModIntro; first set_solver.
+  iSplit; [done|]; iNext; iIntros (e2 σ2 efs ?).
   destruct (Hstep σ1 e2 σ2 efs); auto; subst.
   iMod "Hclose" as "_". iFrame "Hσ". iMod "H". iApply "H"; auto.
 Qed.
 
-Lemma wp_lift_pure_stuck `{Inhabited (state Λ)} E Φ e :
-  (∀ σ, ¬ progressive e σ) →
-  True ⊢ WP e @ E ?{{ Φ }}.
-Proof.
-  iIntros (Hstuck) "_". iApply wp_lift_stuck.
-  - destruct(to_val e) as [v|] eqn:He; last done.
-    exfalso. apply (Hstuck inhabitant). left. by exists v.
-  - iIntros (σ) "_". iMod (fupd_intro_mask' E ∅) as "_".
-    by set_solver. by auto.
-Qed.
-
 (* Atomic steps don't need any mask-changing business here, one can
    use the generic lemmas here. *)
-Lemma wp_lift_atomic_step {s E Φ} e1 :
+Lemma wp_lift_atomic_step {E Φ} e1 :
   to_val e1 = None →
   (∀ σ1, state_interp σ1 ={E}=∗
-    ⌜if s is not_stuck then reducible e1 σ1 else True⌝ ∗
+    ⌜reducible e1 σ1⌝ ∗
     ▷ ∀ e2 σ2 efs, ⌜prim_step e1 σ1 e2 σ2 efs⌝ ={E}=∗
       state_interp σ2 ∗
-      default False (to_val e2) Φ ∗ [∗ list] ef ∈ efs, WP ef @ s; ⊤ {{ _, True }})
-  ⊢ WP e1 @ s; E {{ Φ }}.
+      default False (to_val e2) Φ ∗ [∗ list] ef ∈ efs, WP ef {{ _, True }})
+  ⊢ WP e1 @ E {{ Φ }}.
 Proof.
-  iIntros (?) "H". iApply (wp_lift_step s E _ e1)=>//; iIntros (σ1) "Hσ1".
+  iIntros (?) "H". iApply (wp_lift_step E _ e1)=>//; iIntros (σ1) "Hσ1".
   iMod ("H" $! σ1 with "Hσ1") as "[$ H]".
   iMod (fupd_intro_mask' E ∅) as "Hclose"; first set_solver.
   iModIntro; iNext; iIntros (e2 σ2 efs) "%". iMod "Hclose" as "_".
@@ -83,36 +57,32 @@ Proof.
   by iApply wp_value.
 Qed.
 
-Lemma wp_lift_pure_det_step `{Inhabited (state Λ)} {s E E' Φ} e1 e2 efs :
-  to_val e1 = None →
-  (∀ σ1, if s is not_stuck then reducible e1 σ1 else true) →
+Lemma wp_lift_pure_det_step `{Inhabited (state Λ)} {E E' Φ} e1 e2 efs :
+  (∀ σ1, reducible e1 σ1) →
   (∀ σ1 e2' σ2 efs', prim_step e1 σ1 e2' σ2 efs' → σ1 = σ2 ∧ e2 = e2' ∧ efs = efs')→
-  (|={E,E'}▷=> WP e2 @ s; E {{ Φ }} ∗ [∗ list] ef ∈ efs, WP ef @ s; ⊤ {{ _, True }})
-  ⊢ WP e1 @ s; E {{ Φ }}.
+  (|={E,E'}▷=> WP e2 @ E {{ Φ }} ∗ [∗ list] ef ∈ efs, WP ef {{ _, True }})
+  ⊢ WP e1 @ E {{ Φ }}.
 Proof.
-  iIntros (?? Hpuredet) "H". iApply (wp_lift_pure_step s E E'); try done.
+  iIntros (? Hpuredet) "H". iApply (wp_lift_pure_step E); try done.
   { by intros; eapply Hpuredet. }
   iApply (step_fupd_wand with "H"); iIntros "H".
   by iIntros (e' efs' σ (_&->&->)%Hpuredet).
 Qed.
 
-Lemma wp_pure_step_fupd `{Inhabited (state Λ)} s E E' e1 e2 φ Φ :
+Lemma wp_pure_step_fupd `{Inhabited (state Λ)} E E' e1 e2 φ Φ :
   PureExec φ e1 e2 →
   φ →
-  (|={E,E'}▷=> WP e2 @ s; E {{ Φ }}) ⊢ WP e1 @ s; E {{ Φ }}.
+  (|={E,E'}▷=> WP e2 @ E {{ Φ }}) ⊢ WP e1 @ E {{ Φ }}.
 Proof.
   iIntros ([??] Hφ) "HWP".
-  iApply (wp_lift_pure_det_step with "[HWP]").
-  - apply (reducible_not_val _ inhabitant). by auto.
-  - destruct s; naive_solver.
-  - naive_solver.
-  - by rewrite big_sepL_nil right_id.
+  iApply (wp_lift_pure_det_step with "[HWP]"); [eauto|naive_solver|].
+  rewrite big_sepL_nil right_id //.
 Qed.
 
-Lemma wp_pure_step_later `{Inhabited (state Λ)} s E e1 e2 φ Φ :
+Lemma wp_pure_step_later `{Inhabited (state Λ)} E e1 e2 φ Φ :
   PureExec φ e1 e2 →
   φ →
-  ▷ WP e2 @ s; E {{ Φ }} ⊢ WP e1 @ s; E {{ Φ }}.
+  ▷ WP e2 @ E {{ Φ }} ⊢ WP e1 @ E {{ Φ }}.
 Proof.
   intros ??. rewrite -wp_pure_step_fupd //. rewrite -step_fupd_intro //.
 Qed.
